small modifies

src/proofs/no_slashable_attestations/supporting_lemmas/dv_next_preserves_ind_inv/invs_dv_next_4.dfy
@@ -546,7 +546,7 @@ module Invs_DV_Next_4
     
     // TODO
 
-    predicate undecided_att_duty_in_queue(process: DVCState) 
+    predicate first_queued_att_duty_was_decided_or_ready_to_be_served(process: DVCState) 
     {
         && process.attestation_duties_queue != [] 
         &&  (
@@ -555,102 +555,138 @@ module Invs_DV_Next_4
             ) 
     }
 
-    predicate first_queued_att_duty_was_decided(process: DVCState) 
+    predicate first_queued_att_duty_was_decided(process: DVCState)
     {
+        process.attestation_duties_queue != [] 
+        ==>
         process.attestation_duties_queue[0].slot in process.future_att_consensus_instances_already_decided.Keys
     }
 
-    lemma lem_concl_exists_honest_dvc_that_sent_att_share_for_submitted_att_new_f_check_for_next_queued_duty(
-        process: DVCState,
-        s': DVCState,
+    function f_dequeue_attestation_duties_queue(process: DVCState): DVCState
+    requires first_queued_att_duty_was_decided_or_ready_to_be_served(process)
+    requires first_queued_att_duty_was_decided(process)
+    {
+        var queue_head := process.attestation_duties_queue[0];
+        var new_attestation_slashing_db := f_update_attestation_slashing_db(process.attestation_slashing_db, process.future_att_consensus_instances_already_decided[queue_head.slot]);
+        var ret_process := 
+            process.(
+                        attestation_duties_queue := process.attestation_duties_queue[1..],
+                        future_att_consensus_instances_already_decided := process.future_att_consensus_instances_already_decided - {queue_head.slot},
+                        attestation_slashing_db := new_attestation_slashing_db,
+                        attestation_consensus_engine_state := updateConsensusInstanceValidityCheck(
+                            process.attestation_consensus_engine_state,
+                            new_attestation_slashing_db
+                        )
+            );
+        ret_process
+    }
+
+    lemma lem_concl_exists_honest_dvc_that_sent_att_share_for_submitted_att_new_f_dequeue_attestation_duties_queue(
+        process: DVCState,        
         dv: DVState,
         n: BLSPubkey,
-        index_next_attestation_duty_to_be_served: nat
+        index_next_attestation_duty_to_be_served: nat,
+        s_mod: DVCState
     )
     requires f_check_for_next_queued_duty.requires(process)
-    requires s' == f_check_for_next_queued_duty(process).state   
     requires inv_inv_decided_values_of_previous_duties_are_known_body_body_new(dv, n, process)
-    requires inv_exists_decided_value_for_every_duty_before_queued_duties_body_body(dv, n, process)
+    requires inv_exists_decided_value_for_every_duty_before_queued_duties_body_body(dv, n, process)    
     requires inv_db_of_validity_predicate_contains_all_previous_decided_values_b_body_body(dv, n, process, index_next_attestation_duty_to_be_served)
     requires inv_g_d_a_body_body(dv, n, process)
     requires inv_attestation_duty_queue_is_ordered_3_body_body(dv, n, process)  
-
-    ensures inv_inv_decided_values_of_previous_duties_are_known_body_body_new(dv, n, s');
-    decreases process.attestation_duties_queue
+    requires first_queued_att_duty_was_decided_or_ready_to_be_served(process)
+    requires first_queued_att_duty_was_decided(process)
+    requires s_mod == f_dequeue_attestation_duties_queue(process)
+    ensures ( && |s_mod.attestation_duties_queue| > 0 
+              && !s_mod.current_attestation_duty.isPresent() )
+                    ==> inv_exists_decided_value_for_every_duty_before_queued_duties_body_body(dv, n, s_mod)
     {
-        if  undecided_att_duty_in_queue(process)
+        if  && |s_mod.attestation_duties_queue| > 0 
+              && !s_mod.current_attestation_duty.isPresent()
         {
-            if  first_queued_att_duty_was_decided(process)
+        forall an |
+            && an in dv.sequence_attestation_duties_to_be_served.Values 
+            && an.node == n 
+            && an.attestation_duty.slot < s_mod.attestation_duties_queue[0].slot
+        ensures 
+            var slot := an.attestation_duty.slot;
+            && dv.consensus_on_attestation_data[slot].decided_value.isPresent()
+            && construct_SlashingDBAttestation_from_att_data(dv.consensus_on_attestation_data[slot].decided_value.safe_get()) in s_mod.attestation_slashing_db     
+        ;                          
+        {
+            var slot := an.attestation_duty.slot;
+        
+            if an.attestation_duty.slot < process.attestation_duties_queue[0].slot  
             {
-                var queue_head := process.attestation_duties_queue[0];
-                var new_attestation_slashing_db := f_update_attestation_slashing_db(process.attestation_slashing_db, process.future_att_consensus_instances_already_decided[queue_head.slot]);
-                var s_mod := process.(
-                    attestation_duties_queue := process.attestation_duties_queue[1..],
-                    future_att_consensus_instances_already_decided := process.future_att_consensus_instances_already_decided - {queue_head.slot},
-                    attestation_slashing_db := new_attestation_slashing_db,
-                    attestation_consensus_engine_state := updateConsensusInstanceValidityCheck(
-                        process.attestation_consensus_engine_state,
-                        new_attestation_slashing_db
-                    )                        
-                );
+                assert 
+                    && dv.consensus_on_attestation_data[slot].decided_value.isPresent()
+                    && construct_SlashingDBAttestation_from_att_data(dv.consensus_on_attestation_data[slot].decided_value.safe_get()) in s_mod.attestation_slashing_db     
+                ;
+            }
+            else 
+            {
+                var t :|  dv.sequence_attestation_duties_to_be_served[t] == an;
+                assert process.attestation_duties_queue[0] in process.attestation_duties_queue;
+                var k :|  
+                        && dv.sequence_attestation_duties_to_be_served[k].node == n 
+                        && dv.sequence_attestation_duties_to_be_served[k].attestation_duty == process.attestation_duties_queue[0];
+                assert process.attestation_duties_queue[1] in process.attestation_duties_queue;
+                var l :|  
+                        && dv.sequence_attestation_duties_to_be_served[l].node == n 
+                        && dv.sequence_attestation_duties_to_be_served[l].attestation_duty == process.attestation_duties_queue[1];   
 
-                if  && |s_mod.attestation_duties_queue| > 0 
-                    &&   !s_mod.current_attestation_duty.isPresent()
-                {
-                  
-                    forall an |
-                        && an in dv.sequence_attestation_duties_to_be_served.Values 
-                        && an.node == n 
-                        && an.attestation_duty.slot < s_mod.attestation_duties_queue[0].slot
-                    ensures 
-                        var slot := an.attestation_duty.slot;
-                        && dv.consensus_on_attestation_data[slot].decided_value.isPresent()
-                        && construct_SlashingDBAttestation_from_att_data(dv.consensus_on_attestation_data[slot].decided_value.safe_get()) in s_mod.attestation_slashing_db     
-                    ;                          
-                    {
-                        var slot := an.attestation_duty.slot;
-                   
-                        if an.attestation_duty.slot < process.attestation_duties_queue[0].slot  
-                        {
-                            assert 
-                                && dv.consensus_on_attestation_data[slot].decided_value.isPresent()
-                                && construct_SlashingDBAttestation_from_att_data(dv.consensus_on_attestation_data[slot].decided_value.safe_get()) in s_mod.attestation_slashing_db     
-                            ;
-                        }
-                        else 
-                        {
-                            var t :|  dv.sequence_attestation_duties_to_be_served[t] == an;
-                            assert process.attestation_duties_queue[0] in process.attestation_duties_queue;
-                            var k :|  
-                                    && dv.sequence_attestation_duties_to_be_served[k].node == n 
-                                    && dv.sequence_attestation_duties_to_be_served[k].attestation_duty == process.attestation_duties_queue[0];
-                            assert process.attestation_duties_queue[1] in process.attestation_duties_queue;
-                            var l :|  
-                                    && dv.sequence_attestation_duties_to_be_served[l].node == n 
-                                    && dv.sequence_attestation_duties_to_be_served[l].attestation_duty == process.attestation_duties_queue[1];   
+                lem_inv_attestation_duty_queue_is_ordered_3_body_body(
+                    dv,
+                    n,
+                    process,
+                    1,
+                    k,
+                    l,
+                    t
+                ); 
 
-                            lem_inv_attestation_duty_queue_is_ordered_3_body_body(
-                                dv,
-                                n,
-                                process,
-                                1,
-                                k,
-                                l,
-                                t
-                            ); 
+            
+                assert 
+                    && dv.consensus_on_attestation_data[slot].decided_value.isPresent()
+                    && construct_SlashingDBAttestation_from_att_data(dv.consensus_on_attestation_data[slot].decided_value.safe_get()) in s_mod.attestation_slashing_db     
+                ;
+                
+            }
+        }
+        }
+    }
 
-                        
-                            assert 
-                                && dv.consensus_on_attestation_data[slot].decided_value.isPresent()
-                                && construct_SlashingDBAttestation_from_att_data(dv.consensus_on_attestation_data[slot].decided_value.safe_get()) in s_mod.attestation_slashing_db     
-                            ;
-                            
-                        }
-                    }                  
-                }
-                assert inv_exists_decided_value_for_every_duty_before_queued_duties_body_body(dv, n, s_mod);
-
-                forall i: nat, k, l, t  |
+    lemma lem_concl_exists_honest_dvc_that_sent_att_share_for_submitted_att_new_f_dequeue_attestation_duties_queue_helper1(
+        process: DVCState,        
+        dv: DVState,
+        n: BLSPubkey,
+        index_next_attestation_duty_to_be_served: nat,
+        s_mod: DVCState
+    )
+    requires f_check_for_next_queued_duty.requires(process)
+    requires inv_inv_decided_values_of_previous_duties_are_known_body_body_new(dv, n, process)
+    requires inv_exists_decided_value_for_every_duty_before_queued_duties_body_body(dv, n, process)    
+    requires inv_db_of_validity_predicate_contains_all_previous_decided_values_b_body_body(dv, n, process, index_next_attestation_duty_to_be_served)
+    requires inv_g_d_a_body_body(dv, n, process)
+    requires inv_attestation_duty_queue_is_ordered_3_body_body(dv, n, process)  
+    requires first_queued_att_duty_was_decided_or_ready_to_be_served(process)
+    requires first_queued_att_duty_was_decided(process)
+    requires s_mod == f_dequeue_attestation_duties_queue(process)
+    
+    ensures forall i: nat, k, l, t  ::
+                inv_attestation_duty_queue_is_ordered_3_body_body_premise(
+                        dv,
+                        n, 
+                        s_mod,
+                        i,
+                        k, 
+                        l, 
+                        t
+                    )
+                ==> 
+                s_mod.attestation_duties_queue[i-1].slot == dv.sequence_attestation_duties_to_be_served[t].attestation_duty.slot      
+    {
+        forall i: nat, k, l, t  |
                     inv_attestation_duty_queue_is_ordered_3_body_body_premise(
                         dv,
                         n, 
@@ -678,9 +714,30 @@ module Invs_DV_Next_4
                         l, 
                         t                        
                     );
-                }   
+                } 
+    }
 
-                forall ad  |
+    lemma lem_concl_exists_honest_dvc_that_sent_att_share_for_submitted_att_new_f_dequeue_attestation_duties_queue_helper2(
+        process: DVCState,        
+        dv: DVState,
+        n: BLSPubkey,
+        index_next_attestation_duty_to_be_served: nat,
+        s_mod: DVCState
+    )
+    requires f_check_for_next_queued_duty.requires(process)
+    requires inv_inv_decided_values_of_previous_duties_are_known_body_body_new(dv, n, process)
+    requires inv_exists_decided_value_for_every_duty_before_queued_duties_body_body(dv, n, process)    
+    requires inv_db_of_validity_predicate_contains_all_previous_decided_values_b_body_body(dv, n, process, index_next_attestation_duty_to_be_served)
+    requires inv_g_d_a_body_body(dv, n, process)
+    requires inv_attestation_duty_queue_is_ordered_3_body_body(dv, n, process)  
+    requires first_queued_att_duty_was_decided_or_ready_to_be_served(process)
+    requires first_queued_att_duty_was_decided(process)
+    requires s_mod == f_dequeue_attestation_duties_queue(process)
+    ensures  forall ad  ::
+                    ad in s_mod.attestation_duties_queue
+                ==> ad in process.attestation_duties_queue
+    {
+        forall ad  |
                     && ad in s_mod.attestation_duties_queue
                 ensures ad in process.attestation_duties_queue
                 {
@@ -688,6 +745,60 @@ module Invs_DV_Next_4
                                 && s_mod.attestation_duties_queue[i] == ad;
                     assert ad in process.attestation_duties_queue;
                 }
+    }
+
+    lemma lem_concl_exists_honest_dvc_that_sent_att_share_for_submitted_att_new_f_check_for_next_queued_duty(
+        process: DVCState,
+        s': DVCState,
+        dv: DVState,
+        n: BLSPubkey,
+        index_next_attestation_duty_to_be_served: nat
+    )
+    requires f_check_for_next_queued_duty.requires(process)
+    requires s' == f_check_for_next_queued_duty(process).state   
+    requires inv_inv_decided_values_of_previous_duties_are_known_body_body_new(dv, n, process)
+    requires inv_exists_decided_value_for_every_duty_before_queued_duties_body_body(dv, n, process)
+    requires inv_db_of_validity_predicate_contains_all_previous_decided_values_b_body_body(dv, n, process, index_next_attestation_duty_to_be_served)
+    requires inv_g_d_a_body_body(dv, n, process)
+    requires inv_attestation_duty_queue_is_ordered_3_body_body(dv, n, process)  
+
+    ensures inv_inv_decided_values_of_previous_duties_are_known_body_body_new(dv, n, s');
+    decreases process.attestation_duties_queue
+    {
+        if  first_queued_att_duty_was_decided_or_ready_to_be_served(process)
+        {
+            if  first_queued_att_duty_was_decided(process)
+            {
+                var s_mod := f_dequeue_attestation_duties_queue(process);
+
+                if  && |s_mod.attestation_duties_queue| > 0 
+                    && !s_mod.current_attestation_duty.isPresent()
+                {
+                    lem_concl_exists_honest_dvc_that_sent_att_share_for_submitted_att_new_f_dequeue_attestation_duties_queue(
+                        process,
+                        dv,
+                        n,
+                        index_next_attestation_duty_to_be_served,
+                        s_mod
+                    );                                      
+                }
+                assert inv_exists_decided_value_for_every_duty_before_queued_duties_body_body(dv, n, s_mod);
+
+                lem_concl_exists_honest_dvc_that_sent_att_share_for_submitted_att_new_f_dequeue_attestation_duties_queue_helper1(
+                        process,
+                        dv,
+                        n,
+                        index_next_attestation_duty_to_be_served,
+                        s_mod
+                );     
+
+                lem_concl_exists_honest_dvc_that_sent_att_share_for_submitted_att_new_f_dequeue_attestation_duties_queue_helper2(
+                        process,
+                        dv,
+                        n,
+                        index_next_attestation_duty_to_be_served,
+                        s_mod
+                );   
                     // ::
                     // exists i: nat :: 
                     //     && i < index_next_attestation_duty_to_be_served
